libcrux-ml-kem/proofs/fstar/extraction/Libcrux_ml_kem.Vector.Portable.Ntt.fsti
@@ -105,7 +105,13 @@ val inv_ntt_layer_1_step
       (ensures
         fun result ->
           let result:Libcrux_ml_kem.Vector.Portable.Vector_type.t_PortableVector = result in
-          Spec.Utils.is_i16b_array 3328 result.f_elements)
+          Spec.Utils.is_i16b_array 3328 result.f_elements /\
+          Spec.Utils.inv_ntt_layer_1_butterfly_post vec.f_elements
+            result.f_elements
+            zeta0
+            zeta1
+            zeta2
+            zeta3)
 
 val inv_ntt_layer_2_step
       (vec: Libcrux_ml_kem.Vector.Portable.Vector_type.t_PortableVector)
@@ -117,7 +123,8 @@ val inv_ntt_layer_2_step
       (ensures
         fun result ->
           let result:Libcrux_ml_kem.Vector.Portable.Vector_type.t_PortableVector = result in
-          Spec.Utils.is_i16b_array 3328 result.f_elements)
+          Spec.Utils.is_i16b_array 3328 result.f_elements /\
+          Spec.Utils.inv_ntt_layer_2_butterfly_post vec.f_elements result.f_elements zeta0 zeta1)
 
 val inv_ntt_layer_3_step
       (vec: Libcrux_ml_kem.Vector.Portable.Vector_type.t_PortableVector)
@@ -127,7 +134,8 @@ val inv_ntt_layer_3_step
       (ensures
         fun result ->
           let result:Libcrux_ml_kem.Vector.Portable.Vector_type.t_PortableVector = result in
-          Spec.Utils.is_i16b_array 3328 result.f_elements)
+          Spec.Utils.is_i16b_array 3328 result.f_elements /\
+          Spec.Utils.inv_ntt_layer_3_butterfly_post vec.f_elements result.f_elements zeta)
 
 let ntt_multiply_binomials_post
       (a b: Libcrux_ml_kem.Vector.Portable.Vector_type.t_PortableVector)
